starting to concretize spec (No Admitted Defs or Typeclasses)

src/AbstractedTypes.v
@@ -1,7 +1,9 @@
-Require Import EqClass.
+(* Require Import EqClass. *)
 
-Definition ID_Type : Set. Admitted.
+Definition ID_Type := nat. (* : Set. Admitted. *)
 
+(*
 Global Instance Eq_Class_ID_Type : EqClass ID_Type. Admitted.
+*)
 
-Definition min_id_type : ID_Type. Admitted.
+Definition min_id_type : ID_Type := O. (* .Admitted. *)
